Apply code reviews

ArchSemArm/VMPromising.v
@@ -388,7 +388,6 @@ Definition strict_regs : gset reg :=
        SP_EL1;
        SP_EL2;
        SP_EL3;
-       PSTATE;
        ELR_EL1;
        ELR_EL2;
        ELR_EL3;
@@ -414,6 +413,15 @@ Definition relaxed_regs : gset reg :=
        VBAR_EL2;
        VBAR_EL3;
        VTTBR_EL2]@{reg}.
+
+Definition ttbrs : gset reg :=
+  list_to_set [
+    TTBR0_EL1;
+    TTBR0_EL2;
+    TTBR0_EL3;
+    TTBR1_EL1;
+    TTBR1_EL2;
+    VTTBR_EL2]@{reg}.
 
 (** Determine if input register is an unknown register from the architecture *)
 Definition is_reg_unknown (r : reg) : Prop :=
@@ -709,8 +717,15 @@ Definition va_to_vpn {n : N} (va : bv 64) : bv n :=
   bv_extract 12 n va.
 
 Definition prefix_to_va {n : N} (is_upper : bool) (p : bv n) : bv 64 :=
-  let varange_bit := if is_upper then (bv_1 16) else (bv_0 16) in
-  bv_concat 64 varange_bit (bv_concat 48 p (bv_0 (48 - n))).
+  let varange_bits : bv 16 := if is_upper then (-1)%bv else 0%bv in
+  let padding := bv_0 (48 - n) in
+  bv_concat 64 varange_bits (bv_concat 48 p padding).
+
+Definition is_upper_va (va : bv 64) : option bool :=
+  let top_bits := bv_extract 48 16 va in
+  if top_bits =? (-1)%bv then Some true
+  else if top_bits =? 0%bv then Some false
+  else None.
 
 Definition level_prefix {n : N} (va : bv n) (lvl : Level) : prefix lvl :=
   bv_extract (12 + 9 * (3 - lvl)) (9 * (lvl + 1)) va.
@@ -741,9 +756,9 @@ Definition is_valid (e : val) : Prop :=
 Instance Decision_is_valid (e : val) : Decision (is_valid e).
 Proof. unfold_decide. Defined.
 
-Definition is_table (e : val) : Prop :=
-  (bv_extract 0 2 e) = 3%bv.
-Instance Decision_is_table (e : val) : Decision (is_table e).
+Definition is_table (lvl : Level) (e : val) : Prop :=
+  lvl ≠ leaf_lvl ∧ (bv_extract 0 2 e) = 3%bv.
+Instance Decision_is_table (lvl : Level) (e : val) : Decision (is_table lvl e).
 Proof. unfold_decide. Defined.
 
 Definition is_block (e : val) : Prop :=
@@ -761,6 +776,20 @@ Definition is_global (lvl : Level) (e : val) : Prop :=
 Instance Decision_is_global (lvl : Level) (e : val) : Decision (is_global lvl e).
 Proof. unfold_decide. Defined.
 
+Definition allow_write (lvl : Level) (e : val) : Prop :=
+  let ap := if decide (is_table lvl e) then (bv_extract 61 2 e)
+            else (bv_extract 6 2 e) in
+  (bv_extract 1 1 ap) = 0%bv.
+Instance Decision_allow_write (lvl : Level) (e : val) : Decision (allow_write lvl e).
+Proof. unfold_decide. Defined.
+
+Definition oa_lo (lvl : Level) : N := (12 + (3 - lvl) * 9)%N.
+
+Definition oa_size (lvl : Level) : N := 48 - (oa_lo lvl).
+
+Definition output_addr (lvl : Level) (e : val) : bv (oa_size lvl) :=
+  bv_extract (oa_lo lvl) (oa_size lvl) e.
+
 (** * TLB ***)
 
 Module TLB.
@@ -768,10 +797,12 @@ Module TLB.
   Module NDCtxt.
     Record t (lvl : Level) :=
       make {
+          is_upper : bool;
           va : prefix lvl;
           asid : option (bv 16);
         }.
     Arguments make {_} _ _.
+    Arguments is_upper {_}.
     Arguments va {_}.
     Arguments asid {_}.
 
@@ -783,8 +814,8 @@ Module TLB.
 
     #[global] Instance count lvl : Countable (t lvl).
     Proof.
-      eapply (inj_countable' (fun ndc => (va ndc, asid ndc))
-                        (fun x => make x.1 x.2)).
+      eapply (inj_countable' (fun ndc => (is_upper ndc, va ndc, asid ndc))
+                        (fun x => make x.1.1 x.1.2 x.2)).
       abstract sauto.
     Defined.
   End NDCtxt.
@@ -793,22 +824,19 @@ Module TLB.
     Definition t := {lvl : Level & NDCtxt.t lvl}.
     Definition lvl : t -> Level := projT1.
     Definition nd (ctxt : t) : NDCtxt.t (lvl ctxt) := projT2 ctxt.
+    Definition is_upper (ctxt : t) : bool := NDCtxt.is_upper (nd ctxt).
     Definition va (ctxt : t) : prefix (lvl ctxt) := NDCtxt.va (nd ctxt).
     Definition asid (ctxt : t) : option (bv 16) := NDCtxt.asid (nd ctxt).
   End Ctxt.
   #[export] Typeclasses Transparent Ctxt.t.
 
   Module Entry.
-    Record t (lvl : Level) :=
+    Record t {lvl : Level} :=
       make {
-        is_upper : bool;
         val_ttbr : val;
         ptes : vec val (S lvl);
       }.
-    Arguments make {_} _ _ _.
-    Arguments is_upper {_}.
-    Arguments val_ttbr {_}.
-    Arguments ptes {_}.
+    Arguments t : clear implicits.
 
     #[global] Instance eq_dec lvl : EqDecision (t lvl).
     Proof. solve_decision. Defined.
@@ -818,8 +846,8 @@ Module TLB.
 
     #[global] Instance count lvl : Countable (t lvl).
     Proof.
-      eapply (inj_countable' (fun ent => (is_upper ent, val_ttbr ent, ptes ent))
-                        (fun x => make x.1.1 x.1.2 x.2)).
+      eapply (inj_countable' (fun ent => (val_ttbr ent, ptes ent))
+                        (fun x => make lvl x.1 x.2)).
       abstract sauto.
     Defined.
 
@@ -828,8 +856,8 @@ Module TLB.
     Program Definition append {lvl clvl : Level}
         (tlbe : t lvl)
         (pte : val)
-        (CHILD : lvl + 1 = clvl) : t clvl :=
-      make tlbe.(is_upper) tlbe.(val_ttbr) (ctrans _ (tlbe.(ptes) +++ [#pte])).
+        (CHILD : lvl + 1 = clvl) : @t clvl :=
+      make _ tlbe.(val_ttbr) (ctrans _ (tlbe.(ptes) +++ [#pte])).
     Solve All Obligations with lia.
   End Entry.
   Export (hints) Entry.
@@ -851,7 +879,7 @@ Module TLB.
     #[global] Typeclasses Transparent T.
     Definition t := hvec T.
 
-    Definition init : t := hvec_func (fun lvl => ∅).
+    Definition init : t := hvec_func (λ lvl, ∅).
 
     Definition get (ctxt : Ctxt.t) (vatlb : t) :
         gset (Entry.t (Ctxt.lvl ctxt)) :=
@@ -859,7 +887,7 @@ Module TLB.
 
     Definition getFE (ctxt : Ctxt.t) (vatlb : t) : gset (FE.t) :=
       get ctxt vatlb
-      |> set_map (fun (e : Entry.t (Ctxt.lvl ctxt)) => existT ctxt e).
+      |> set_map (existT ctxt).
 
     Definition singleton (ctxt : Ctxt.t) (entry : Entry.t (Ctxt.lvl ctxt)) : t :=
       hset (Ctxt.lvl ctxt) {[(Ctxt.nd ctxt) := {[ entry ]}]} init.
@@ -892,15 +920,20 @@ Module TLB.
 
     Definition setFEs (ctxt : Ctxt.t)
         (entries : gset (Entry.t (Ctxt.lvl ctxt))) (vatlb : t) : t :=
-      hset (Ctxt.lvl ctxt) {[(Ctxt.nd ctxt) := entries]} vatlb.
+      let lvl := Ctxt.lvl ctxt in
+      let nd := Ctxt.nd ctxt in
+      hset lvl (<[ nd := entries ]> (hget lvl vatlb)) vatlb.
 
     Definition insert (ctxt : Ctxt.t) (entry : Entry.t (Ctxt.lvl ctxt))
         (vatlb : t) : t :=
-      let entries := get ctxt vatlb in
-      hset (Ctxt.lvl ctxt) {[(Ctxt.nd ctxt) := entries ∪ {[ entry ]}]} vatlb.
+      let lvl := Ctxt.lvl ctxt in
+      let nd := Ctxt.nd ctxt in
+      let lvl_map : T lvl := hget lvl vatlb in
+      let entries := (get ctxt vatlb) ∪ {[ entry ]} in
+      hset lvl (<[ nd := entries ]> lvl_map) vatlb.
 
     #[global] Instance empty : Empty t := VATLB.init.
-    #[global] Instance union : Union t := fun x y => hmap2 (fun _ => (∪ₘ)) x y.
+    #[global] Instance union : Union t := λ x y, hmap2 (λ _, (∪ₘ)) x y.
   End VATLB.
   Export (hints) VATLB.
 
@@ -969,12 +1002,12 @@ Module TLB.
       let entry_addr := next_entry_addr val_ttbr va in
       let loc := Loc.from_addr_in entry_addr in
       if (Memory.read_at loc init mem time) is Some (memval, _) then
-        if decide (is_table memval) then
+        if decide (is_table root_lvl memval) then
           let asid := bv_extract 48 16 val_ttbr in
-          let ndctxt := NDCtxt.make va (Some asid) in
+          let ndctxt := NDCtxt.make is_upper va (Some asid) in
           let ctxt := existT root_lvl ndctxt in
           let entry : Entry.t (Ctxt.lvl ctxt) :=
-            Entry.make is_upper val_ttbr ([#memval] : vec val (S root_lvl)) in
+            Entry.make _ val_ttbr ([#memval] : vec val (S root_lvl)) in
           (* add the entry to vatlb only when it is not in the original vatlb *)
           if decide (entry ∉ (VATLB.get ctxt vatlb)) then
             Ok (VATLB.insert ctxt entry vatlb, true)
@@ -998,32 +1031,29 @@ Module TLB.
       (te : Entry.t (Ctxt.lvl ctxt))
       (index : bv 9)
       (ttbr : reg) : result string (VATLB.t * bool) :=
-    (* guard_or "ASID is not active"
-      $ is_active_asid ts (Ctxt.asid ctxt) ttbr time;; *)
-    guard_or "The translation entry is not in the TLB"
-      (te ∈ VATLB.get ctxt vatlb);;
-
-    if decide (¬is_table (Entry.pte te)) then Ok (vatlb, false)
+    let plvl := Ctxt.lvl ctxt in
+    if decide (¬is_table plvl (Entry.pte te)) then Ok (vatlb, false)
     else
       let entry_addr := next_entry_addr (Entry.pte te) index in
       let loc := Loc.from_addr_in entry_addr in
-      '(next_pte, _) ← othrow "The location of the next level address should be read"
-                        $ Memory.read_at loc init mem time;
-      if decide (is_valid next_pte) then
-        match inspect $ child_lvl (Ctxt.lvl ctxt) with
-        | Some clvl eq:e =>
-          let va := next_va ctxt index (child_lvl_add_one _ _ e) in
-          let asid := if bool_decide (is_global clvl next_pte) then None
-                      else Ctxt.asid ctxt in
-          let ndctxt := NDCtxt.make va asid in
-          let ctxt := existT clvl ndctxt in
-          let entry := Entry.append te next_pte (child_lvl_add_one _ _ e) in
-          (* add the entry to vatlb only when it is not in the original vatlb *)
-          if decide (entry ∉ (VATLB.get ctxt vatlb)) then
-            Ok (VATLB.insert ctxt entry vatlb, true)
-          else Ok (vatlb, false)
-        | None eq:_ => mthrow "An intermediate level should have a child level"
-        end
+      if (Memory.read_at loc init mem time) is Some (next_pte, _) then
+        if decide (is_valid next_pte) then
+          match inspect $ child_lvl plvl with
+          | Some clvl eq:e =>
+            let va := next_va ctxt index (child_lvl_add_one _ _ e) in
+            let asid := if bool_decide (is_global clvl next_pte) then None
+                        else Ctxt.asid ctxt in
+            let ndctxt := NDCtxt.make (Ctxt.is_upper ctxt) va asid in
+            let ctxt := existT clvl ndctxt in
+            let entry := Entry.append te next_pte (child_lvl_add_one _ _ e) in
+            (* add the entry to vatlb only when it is not in the original vatlb *)
+            if decide (entry ∉ (VATLB.get ctxt vatlb)) then
+              Ok (VATLB.insert ctxt entry vatlb, true)
+            else Ok (vatlb, false)
+          | None eq:_ => mthrow "An intermediate level should have a child level"
+          end
+        else
+          Ok (vatlb, false)
       else
         Ok (vatlb, false).
 
@@ -1047,11 +1077,12 @@ Module TLB.
         let index := level_index va lvl in
         sregs ← othrow "TTBR should exist in initial state"
                 $ TState.read_sreg_at ts ttbr time;
+        is_upper ← othrow "The register is not TTBR" (is_upper_ttbr ttbr);
         foldlM (λ prev sreg,
           val_ttbr ← othrow "TTBR should be a 64 bit value"
                   $ regval_to_val ttbr sreg.1;
           let asid := bv_extract 48 16 val_ttbr in
-          let ndctxt := NDCtxt.make pva (Some asid) in
+          let ndctxt := NDCtxt.make is_upper pva (Some asid) in
           let ctxt := existT plvl ndctxt in
           (* parent entries should be from the original TLB (in the parent level) *)
           let tes := elements (VATLB.get ctxt tlb.(vatlb)) in
@@ -1064,18 +1095,83 @@ Module TLB.
       end;
     mret $ (TLB.make vatlb_new, is_changed).
 
-  (** Fill TLB entries for [va] through all levels 0–3.
-      - Sequentially calls [va_fill] at each level.
+  (** Fill TLB entries for va through all levels 0–3.
+      - Sequentially calls va_fill at each level.
       - Produces a TLB with the full translation chain if available. *)
-  Definition update (tlb : t)
-      (ts : TState.t)
+  Definition update_for_va (tlb : t) (ts : TState.t)
       (init : Memory.initial)
       (mem : Memory.t)
       (time : nat)
       (va : bv 64)
       (ttbr : reg) : result string (t * bool) :=
     foldlM (λ '(tlb_prev, is_changed_prev) lvl,
-      '(tlb_new, is_changed) ← va_fill tlb_prev ts init mem time lvl va ttbr;
+      '(tlb_new, is_changed) ←
+        va_fill tlb_prev ts init mem time lvl va ttbr;
+      mret (tlb_new, is_changed || is_changed_prev)
+    ) (tlb, false) (enum Level).
+
+  Definition traverse_root (vatlb : VATLB.t) (ts : TState.t)
+        (init : Memory.initial)
+        (mem : Memory.t)
+        (time : nat)
+        (ttbr : reg) : result string (VATLB.t * bool) :=
+    foldlM (λ '(vatlb_prev, is_changed_prev) i,
+      '(vatlb_new, is_changed) ←
+        va_fill_root vatlb_prev ts init mem time (Z_to_bv 9 i) ttbr;
+      mret (vatlb_new, is_changed || is_changed_prev)
+    ) (vatlb, false) (seqZ 0 512).
+
+  Definition traverse_lvl (vatlb : VATLB.t) (ts : TState.t)
+        (init : Memory.initial)
+        (mem : Memory.t)
+        (time : nat)
+        (ctxt : Ctxt.t)
+        (ttbr : reg) : result string (VATLB.t * bool) :=
+    let table_entries := elements (VATLB.get ctxt vatlb) in
+    foldlM (λ prev table,
+      foldlM (λ '(vatlb_prev, is_changed_prev) i,
+        '(vatlb_new, is_changed_new) ←
+          va_fill_lvl vatlb_prev ts init mem time ctxt table (Z_to_bv 9 i) ttbr;
+        mret (vatlb_new, is_changed_new || is_changed_prev)
+      ) prev (seqZ 0 512)
+    ) (vatlb, false) table_entries.
+
+  (** Traverse the page table for [ttbr] and build a TLB for all vas
+      along with the boolean value that returns (tlb, is_changed, ctxts).
+      is_changed is true  when there are new VATLB entries *)
+  Definition traverse (tlb : t) (ts : TState.t)
+      (init : Memory.initial)
+      (mem : Memory.t)
+      (time : nat)
+      (lvl : Level)
+      (ttbr : reg) : result string (t * bool) :=
+    '(vatlb_new, is_changed) ←
+      match parent_lvl lvl with
+      | None => traverse_root tlb.(vatlb) ts init mem time ttbr
+      | Some plvl =>
+        let pctxts := remove_dups $
+                    omap (λ fe,
+                          if decide (FE.lvl fe = plvl)
+                            then Some (FE.ctxt fe)
+                            else None) (elements tlb.(vatlb)) in
+        foldlM (λ '(vatlb, is_changed_prev) pctxt,
+          '(vatlb_new, is_changed) ←
+            traverse_lvl vatlb ts init mem time pctxt ttbr;
+          mret (vatlb_new, is_changed || is_changed_prev)
+        ) (tlb.(vatlb), false) pctxts
+      end;
+    mret $ (TLB.make vatlb_new, is_changed).
+
+  (** Fill TLB entries for all vas through all levels 0–3.
+      - Sequentially calls traverse at each level.
+      - Produces a TLB with the full translation chain if available. *)
+  Definition update_all (tlb : t) (ts : TState.t)
+        (init : Memory.initial)
+        (mem : Memory.t)
+        (time : nat)
+        (ttbr : reg) : result string (t * bool) :=
+    foldlM (λ '(tlb_prev, is_changed_prev) lvl,
+      '(tlb_new, is_changed) ← traverse tlb_prev ts init mem time lvl ttbr;
       mret (tlb_new, is_changed || is_changed_prev)
     ) (tlb, false) (enum Level).
 
@@ -1127,10 +1223,10 @@ Module TLB.
   Definition tlbi_apply (tlbi : TLBI.t) (tlb : t) : t :=
     set vatlb (filter (λ '(existT ctxt te), ¬ affects tlbi ctxt te)) tlb.
 
-  (** Get the unique TLB states from [time_prev] to [time_prev + cnt]
+  (** Get the unique TLB states for one [va] from [time_prev] to [time_prev + cnt]
       along with their views as a [list (t * nat)].
       The list is sorted in descending order by timestamp. *)
-  Fixpoint unique_snapshots_between (ts : TState.t) (mem_init : Memory.initial)
+  Fixpoint unique_snapshots_for_va_between (ts : TState.t) (mem_init : Memory.initial)
                        (mem : Memory.t)
                        (tlb_prev : t)
                        (time_prev cnt : nat)
@@ -1147,32 +1243,76 @@ Module TLB.
         | Some ev =>
             (* always true if tlbi is applied *)
             let (tlb_inv, is_changed_by_tlbi) :=
-              if ev is Ev.Tlbi tlbi then (tlbi_apply tlbi tlb_prev, true) else (tlb_prev, false)
+              if ev is Ev.Tlbi tlbi
+              then (tlbi_apply tlbi tlb_prev, true)
+              else (tlb_prev, false)
             in
-            '(tlb, is_changed) ← update tlb_inv ts mem_init mem time_cur va ttbr;
+            '(tlb, is_changed) ← update_for_va tlb_inv ts mem_init mem time_cur va ttbr;
             mret (tlb, is_changed || is_changed_by_tlbi)
         | None => mret (init, false)
         end;
       let acc :=
-        match is_changed with
-        | true => (tlb, time_cur) :: acc
-        | false => acc
-        end in
-      unique_snapshots_between
+        if (is_changed : bool) then (tlb, time_cur) :: acc else acc in
+      unique_snapshots_for_va_between
         ts mem_init mem tlb time_cur ccnt va ttbr acc
     end.
 
-  (** Get the unique TLB states up until the timestamp [time]
+  (** Get the unique TLB states for one [va] up until the timestamp [time]
       along with their views as a [list (TLB.t * nat)].
       The list is sorted in descending order by timestamp. *)
-  Definition unique_snapshots_until (ts : TState.t)
+  Definition unique_snapshots_for_va_until (ts : TState.t)
                        (mem_init : Memory.initial)
                        (mem : Memory.t)
                        (time : nat)
                        (va : bv 64)
                        (ttbr : reg) : result string (list (t * nat)) :=
-    '(tlb, _) ← update init ts mem_init mem 0 va ttbr;
-    unique_snapshots_between ts mem_init mem tlb 0 time va ttbr [(tlb, 0)].
+    '(tlb, _) ← update_for_va init ts mem_init mem 0 va ttbr;
+    unique_snapshots_for_va_between ts mem_init mem tlb 0 time va ttbr [(tlb, 0)].
+
+  (** Get the TLB states for all possible vas from [time_prev] to [time_prev + cnt]
+      along with their views as [list (TLB.t * nat)].
+      The list is sorted in descending order by timestamp. *)
+  Fixpoint unique_snapshots_between (ts : TState.t) (mem_init : Memory.initial)
+                       (mem : Memory.t)
+                       (tlb_prev : t)
+                       (time_prev cnt : nat)
+                       (ttbr : reg)
+                       (acc : list (t * nat)) :
+                      result string (list (t * nat)) :=
+    match cnt with
+    | O => mret acc
+    | S ccnt =>
+      let time_cur := time_prev + 1 in
+      '(tlb, is_changed) ←
+        match mem !! time_cur with
+        | Some ev =>
+            (* always true if tlbi is applied *)
+            let (tlb_inv, is_changed_by_tlbi) :=
+              if ev is Ev.Tlbi tlbi
+              then (tlbi_apply tlbi tlb_prev, true)
+              else (tlb_prev, false)
+            in
+            '(tlb, is_changed) ← update_all tlb_inv ts mem_init mem time_cur ttbr;
+            mret (tlb, is_changed || is_changed_by_tlbi)
+        | None => mret (init, false)
+        end;
+      let acc :=
+        if (is_changed : bool) then (tlb, time_cur) :: acc else acc in
+      unique_snapshots_between
+        ts mem_init mem tlb time_cur ccnt ttbr acc
+    end.
+
+  (** Get the TLB states for all possible vas up until the timestamp [time]
+      along with their views and contexts that can retrieve values from that state
+      as [list (TLB.t * nat)].
+      The list is sorted in descending order by timestamp. *)
+  Definition unique_snapshots_until (ts : TState.t)
+                       (mem_init : Memory.initial)
+                       (mem : Memory.t)
+                       (time : nat)
+                       (ttbr : reg) : result string (list (t * nat)) :=
+    '(tlb, _) ← update_all init ts mem_init mem 0 ttbr;
+    unique_snapshots_between ts mem_init mem tlb 0 time ttbr [(tlb, 0)].
 
   Definition is_te_invalidated_by_tlbi
                 (tlbi : TLBI.t)
@@ -1194,7 +1334,6 @@ Module TLB.
     | (ev, t) :: tl =>
       match ev with
       | Ev.Tlbi tlbi =>
-        let va := prefix_to_va (Entry.is_upper te) (Ctxt.va ctxt) in
         if decide (is_te_invalidated_by_tlbi tlbi tid ctxt te) then
           mret (Some t)
         else
@@ -1228,7 +1367,7 @@ Module TLB.
       mret ((Entry.val_ttbr te), (vec_to_list (Entry.ptes te)), ti)
     end.
 
-  (** Get all the TLB entries and the corresponding TTBR value that
+  (** Get all the TLB entries (including the TTBR value) TTBR value that
       could translate the given VA at the provided level
       and in the provided ASID context.
       Return each TLB entry as a list of descriptors [list val] with
@@ -1239,8 +1378,10 @@ Module TLB.
               (lvl : Level)
               (va : bv 64) (asid : bv 16) :
             result string (list (val * list val * (option nat))) :=
-    let ndctxt_asid := NDCtxt.make (level_prefix va lvl) (Some asid) in
-    let ndctxt_global := NDCtxt.make (level_prefix va lvl) None in
+    is_upper ← othrow ("VA is not in the 48 bits range: " ++ (pretty va))%string
+                (is_upper_va va);
+    let ndctxt_asid := NDCtxt.make is_upper (level_prefix va lvl) (Some asid) in
+    let ndctxt_global := NDCtxt.make is_upper (level_prefix va lvl) None in
     candidates_asid ←
       get_leaf_ptes_with_inv_time_by_ctxt mem tid tlb trans_time lvl ndctxt_asid;
     candidates_global ←
@@ -1277,10 +1418,12 @@ Module TLB.
                 (ttbr : reg) :
         result string (list (val * list val * (option nat))) :=
     if parent_lvl lvl is Some parent_lvl then
-      let ndctxt := NDCtxt.make (level_prefix va parent_lvl) asid in
+      is_upper ← othrow ("VA is not in the range: " ++ (pretty va))%string
+                (is_upper_va va);
+      let ndctxt := NDCtxt.make is_upper (level_prefix va parent_lvl) asid in
       let ctxt := existT parent_lvl ndctxt in
       let tes := VATLB.get ctxt tlb.(TLB.vatlb) in
-      let tes := filter (λ te, is_table (TLB.Entry.pte te)) tes in
+      let tes := filter (λ te, is_table parent_lvl (TLB.Entry.pte te)) tes in
       invalid_ptes ←
         for te in (elements tes) do
           let entry_addr :=
@@ -1376,7 +1519,7 @@ Module TLB.
       candidates ← TLB.lookup mem tid tlb trans_time va asid;
       let new :=
         omap (λ '(val_ttbr, path, ti_opt),
-          if (is_new_entry val_ttbr path ti_opt entries) then
+          if is_new_entry val_ttbr path ti_opt entries then
             Some (val_ttbr, path, trans_time, ti_opt)
           else None
         ) candidates in
@@ -1397,7 +1540,7 @@ Module TLB.
         candidates ← TLB.get_invalid_ptes_with_inv_time ts init mem tid tlb trans_time va asid ttbr;
         let new :=
           omap (λ '(val_ttbr, path, ti_opt),
-            if decide (is_new_entry val_ttbr path ti_opt entries) then
+            if is_new_entry val_ttbr path ti_opt entries then
               Some (val_ttbr, path, trans_time, ti_opt)
             else None
           ) candidates in
@@ -1420,8 +1563,7 @@ Module IIS.
           va : bv 36;
           time : nat;
           root : option {ttbr : reg & reg_type ttbr};
-          remaining : list (bv 64);
-          invalidation : option nat
+          remaining : list (bv 64)
         }.
 
     Definition pop : Exec.t t string (bv 64) :=
@@ -1436,10 +1578,11 @@ Module IIS.
     make {
         strict : view;
         (* The translations results of the latest translation *)
-        trs : option TransRes.t
+        trs : option TransRes.t;
+        inv_time : option nat
       }.
 
-  Definition init : t := make 0 None.
+  Definition init : t := make 0 None None.
 
   (** Add a new view to the IIS *)
   Definition add (v : view) (iis : t) : t :=
@@ -1447,6 +1590,9 @@ Module IIS.
 
   Definition set_trs (tres : TransRes.t) :=
     setv trs (Some tres).
+
+  Definition set_inv_time (ti_opt : option nat) :=
+    setv inv_time ti_opt.
 
 End IIS.
 
@@ -1520,14 +1666,18 @@ Definition run_reg_general_read (reg : reg) (racc : reg_acc) :
 Definition run_reg_trans_read (reg : reg) (racc : reg_acc)
       (trs : IIS.TransRes.t) :
     Exec.t TState.t string (reg_type reg * view) :=
-  guard_or "Translation read during the translation should be implicit"
+  guard_or "Register read during the translation should be implicit"
     (¬ (is_Some racc));;
   root ← othrow "Could not find the translation root: error in translation assumptions"
     (trs.(IIS.TransRes.root));
-  if decide (projT1 root = reg) is left eq then
-    mret (ctrans eq (projT2 root), 0%nat)
+  if decide (root.T1 = reg) is left eq then
+    mret (ctrans eq root.T2, 0%nat)
   else
     ts ← mGet;
+    (* We are only allowed to read registers that are never written during the translation *)
+    guard_or
+      ("The register should niether be relaxed nor strict: " ++ pretty reg)%string
+      $ (reg ∉ strict_regs ∧ reg ∉ relaxed_regs);;
     othrow
       ("Register " ++ pretty reg ++ " unmapped; cannot read")%string
       $ TState.read_reg ts reg.
@@ -1588,18 +1738,14 @@ Definition run_mem_read (addr : address) (macc : mem_acc) (init : Memory.initial
   iis ← mget PPState.iis;
   let vaddr := iis.(IIS.strict) in
   if is_explicit macc then
-    tres_opt ← mget (IIS.trs ∘ PPState.iis);
-    trans_res ← othrow "Explicit access before translation" tres_opt;
-    let invalidation := trans_res.(IIS.TransRes.invalidation) in
     '(view, val) ←
       Exec.liftSt (PPState.state ×× PPState.mem)
-        $ read_mem_explicit loc vaddr invalidation macc init;
+        $ read_mem_explicit loc vaddr iis.(IIS.inv_time) macc init;
     mset PPState.iis $ IIS.add view;;
     mret val
   else if is_ttw macc then
     ts ← mget PPState.state;
-    tres_option ← mget (IIS.trs ∘ PPState.iis);
-    tres ← othrow "TTW read before translation start" tres_option;
+    tres ← othrow "TTW read before translation start" iis.(IIS.trs);
     '(view, val) ←
       read_pte vaddr (ts, tres)
       |> Exec.lift_res_set_full
@@ -1824,31 +1970,34 @@ Definition run_trans_start (trans_start : TranslationStartInfo)
   trans_res ←
     if decide (va_in_range va) then
       ttbr ← mlift $ ttbr_of_regime va trans_start.(TranslationStartInfo_regime);
-      snapshots ← mlift $ TLB.unique_snapshots_until ts init mem vmax_t va ttbr;
+      (* using traversed snapshots also works here *)
+      snapshots ← mlift $ TLB.unique_snapshots_for_va_until ts init mem vmax_t va ttbr;
       valid_entries ← mlift $ TLB.get_valid_entries_from_snapshots snapshots mem tid va asid;
       invalid_entries ← mlift $
         TLB.get_invalid_entries_from_snapshots snapshots ts init mem tid is_ets2 va asid ttbr;
-      (* update IIS with either a valid translation result or a fault *)
-      valid_trs ←
+      (* update IIS with either a valid translation result or an invalid result *)
+      valid_res ←
         for (val_ttbr, path, t, ti) in valid_entries do
           val_ttbr ← othrow
             "TTBR value type does not match with the value from the translation"
             (val_to_regval ttbr val_ttbr);
           let root := (Some (existT ttbr val_ttbr)) in
-          mret $ IIS.TransRes.make (va_to_vpn va) t root path ti
+          let ti := if is_ifetch then ti else None in
+          mret $ (IIS.TransRes.make (va_to_vpn va) t root path, ti)
         end;
-      invalid_trs ←
+      invalid_res ←
         for (val_ttbr, path, t, ti) in invalid_entries do
           val_ttbr ← othrow
             "TTBR value type does not match with the value from the translation"
             (val_to_regval ttbr val_ttbr);
           let root := (Some (existT ttbr val_ttbr)) in
-          mret $ IIS.TransRes.make (va_to_vpn va) t root path ti
+          mret $ (IIS.TransRes.make (va_to_vpn va) t root path, ti)
         end;
-      mchoosel (valid_trs ++ invalid_trs)
+      mchoosel (valid_res ++ invalid_res)
     else
-      mret $ IIS.TransRes.make (va_to_vpn va) vpre_t None [] None;
-  mset PPState.iis $ IIS.set_trs trans_res.
+      mret $ (IIS.TransRes.make (va_to_vpn va) vpre_t None [], None);
+  mset PPState.iis $ IIS.set_trs trans_res.1;;
+  mset PPState.iis $ IIS.set_inv_time trans_res.2.
 
 Definition read_fault_vpre (is_acq : bool)
   (trans_time : nat) : Exec.t (TState.t * IIS.t) string view :=
@@ -1876,7 +2025,7 @@ Definition run_trans_end (trans_end : trans_end) :
     let trans_time := trs.(IIS.TransRes.time) in
     let fault := trans_end.(AddressDescriptor_fault) in
     if decide (fault.(FaultRecord_statuscode) = Fault_None) then
-      mret ()
+      msetv (IIS.trs ∘ snd) None
     else
       is_ets3 ← mlift (ets3 ts);
       if is_ets3 && (trans_time <? (ts.(TState.vrd) ⊔ ts.(TState.vwr)))
@@ -1893,20 +2042,19 @@ Definition run_trans_end (trans_end : trans_end) :
         let is_write := fault.(FaultRecord_access).(AccessDescriptor_write) in
         let is_rel := fault.(FaultRecord_access).(AccessDescriptor_relsc) in
         write_view ← write_fault_vpre is_rel trans_time;
-        mset snd $ IIS.add (view_if is_write write_view)
+        mset snd $ IIS.add (view_if is_write write_view);;
+        msetv (IIS.trs ∘ snd) None
   else
     mthrow "Translation ends with an empty translation".
 
+(* TODO: check translation fault using `fault` and handle other cases *)
 Definition run_take_exception (fault : exn) (vmax_t : view) :
     Exec.t (TState.t * IIS.t) string () :=
   iis ← mget snd;
-  if iis.(IIS.trs) is Some trans_res then
-    match trans_res.(IIS.TransRes.invalidation) with
-    | Some invalidation => run_cse invalidation
-    | None => mret ()
-    end
-  else
-    run_cse vmax_t.
+  match iis.(IIS.inv_time) with
+  | Some inv_time => run_cse inv_time
+  | None => run_cse vmax_t
+  end.
 
 (** Runs an outcome. *)
 Section RunOutcome.
@@ -1940,11 +2088,9 @@ Section RunOutcome.
       addr ← othrow "Address not supported" $ Loc.from_addr addr;
       viio ← mget (IIS.strict ∘ PPState.iis);
       if is_explicit macc then
-        tres_opt ← mget (IIS.trs ∘ PPState.iis);
-        trans_res ← othrow "Explicit access before translation" tres_opt;
-        let invalidation := trans_res.(IIS.TransRes.invalidation) in
+        inv_time ← mget (IIS.inv_time ∘ PPState.iis);
         vpre_opt ← Exec.liftSt (PPState.state ×× PPState.mem) $
-                      write_mem_xcl tid addr viio invalidation macc val;
+                      write_mem_xcl tid addr viio inv_time macc val;
         mret (Ok (), vpre_opt)
       else mthrow "Unsupported non-explicit write"
   | MemWrite _ _ _ => mthrow "Memory write of size other than 8, or with tags"
@@ -1979,6 +2125,136 @@ Section RunOutcome.
     run_outcome out |$> fst.
 
 End RunOutcome.
+
+Section BBM.
+  Context (initmem : memoryMap).
+
+  Definition is_mmu_enabled (ts : TState.t) : result string bool :=
+    '(sctlr, _) ← othrow "SCTLR_EL1 is not set" $
+                    TState.read_reg ts SCTLR_EL1;
+    val_sctlr ← othrow "SCTLR_EL1 should be bv 64" $
+                  regval_to_val SCTLR_EL1 sctlr;
+    Ok ((bv_extract 0 1 val_sctlr) =? 1%bv).
+
+  Definition eq_block_size (lvl : Level) (pte1 pte2 : val) : Prop :=
+    (is_table lvl pte1 ∧ is_table lvl pte2)
+    ∨ (is_block pte1 ∧ is_block pte2)
+    ∨ (lvl = leaf_lvl ∧ is_final lvl pte1 ∧ is_final lvl pte2).
+  Instance Decision_eq_block_size (lvl : Level) (pte1 pte2 : val) :
+    Decision (eq_block_size lvl pte1 pte2).
+  Proof. unfold_decide. Defined.
+
+  Definition is_loc_from_baddr {n : N} (loc : Loc.t) (baddr : bv n) : Prop :=
+    bv_extract (53 - n) n loc = baddr.
+  Instance Decision_is_loc_from_baddr {n : N} (loc : Loc.t) (baddr : bv n) :
+    Decision (is_loc_from_baddr loc baddr).
+  Proof. unfold_decide. Defined.
+
+  Definition timestamp_before_tlbi (mem : Memory.t) : list nat :=
+    omap
+      (λ i,
+        if (mem !! i) is Some ev then
+          if ev is Ev.Tlbi _ then Some (i-1) else None
+        else None) (seq 1 (length mem)).
+
+  Definition same_mem_content (mem : Memory.t) (init : Memory.initial)
+                (time : nat)
+                (lvl : Level)
+                (oa1 oa2 : bv (oa_size lvl))
+                (used_locs : list Loc.t) : bool :=
+    let offset_end := (53 - oa_size lvl)%N in
+    let used_offs :=
+      omap (λ loc,
+        if decide (is_loc_from_baddr loc oa1 ∨ is_loc_from_baddr loc oa2)
+          then Some (bv_extract 0 offset_end loc)
+          else None) used_locs in
+    (* Check if the memory contents derived from two OAs are identical
+        (Assume that locations that are not initialized are 0) *)
+    forallb (λ offs,
+      let loc1 := bv_concat 53 oa1 offs in
+      let loc2 := bv_concat 53 oa2 offs in
+      let res1 := Memory.read_at loc1 init mem time in
+      let res2 := Memory.read_at loc2 init mem time in
+      match res1, res2 with
+      | Some res1, Some res2 => fst res1 =? fst res2
+      | Some res1, None => fst res1 =? 0%bv
+      | None, Some res2 => 0%bv =? fst res2
+      | None, None => true
+      end) used_offs.
+
+  (** Check that the break-before-make (BBM) sequence is respected when modifying
+    a translation table entry. Specifically, two entries derived from the same
+    translation context should not co-exist if any of the following hold:
+
+    - The translation block size changes in granularity (large <-> small)
+    - The output address (OA) mapping changes, and at least one of:
+      - either the old or new mapping permits writes
+      - the memory contents at the new OA differ from those at the old OA
+  *)
+  Definition is_bbm_violated (mem : Memory.t) (init : Memory.initial)
+                (time : nat)
+                (ctxt : TLB.Ctxt.t)
+                (used_locs : list Loc.t)
+                (te1 te2 : TLB.Entry.t (TLB.Ctxt.lvl ctxt)) : bool :=
+    let lvl := TLB.Ctxt.lvl ctxt in
+    let pte1 := TLB.Entry.pte te1 in
+    let pte2 := TLB.Entry.pte te2 in
+    (* When the size of the OA points to are different *)
+    if decide (¬(eq_block_size lvl pte1 pte2)) then true
+    else
+      let oa1 := output_addr lvl pte1 in
+      let oa2 := output_addr lvl pte2 in
+      if (oa1 =? oa2) then false
+      (* When OAs are different *)
+      else if decide (is_table lvl pte1 ∧ is_table lvl pte2) then false
+      else if decide (allow_write lvl pte1 ∨ allow_write lvl pte2) then true
+      else negb (same_mem_content mem init time lvl oa1 oa2 used_locs).
+
+  Definition check_bbm_violation_in_snapshot (mem : Memory.t)
+                (init : Memory.initial)
+                (tlb : TLB.t)
+                (time : nat) : bool :=
+    let used_locs := remove_dups $
+      omap (λ ev,
+        if ev is Ev.Msg msg then Some (Msg.loc msg) else None
+      ) (Memory.cut_before time mem)
+      ++
+      (map fst (map_to_list init)) in
+    let ctxts := remove_dups $ map TLB.FE.ctxt (elements (TLB.vatlb tlb)) in
+    existsb (λ ctxt,
+      let tes := VATLB.get ctxt (TLB.vatlb tlb) in
+      existsb (λ '(te1, te2),
+        if (te1 =? te2) then false
+        else is_bbm_violated mem init time ctxt used_locs te1 te2
+      ) (elements (tes × tes))
+    ) ctxts.
+
+  Definition check_bbm_violation :
+      Exec.t (PPState.t TState.t Ev.t IIS.t) string bool :=
+    ts ← mget PPState.state;
+    mmu_enabled ← mlift $ is_mmu_enabled ts;
+    if (mmu_enabled : bool) then
+      mem ← mget PPState.mem;
+      let initmem := Memory.initial_from_memMap initmem in
+      let max_t := length mem in
+      let ttbrs_to_check :=
+        filter (λ ttbr, is_Some (dmap_lookup ttbr ts.(TState.regs))) ttbrs in
+      let times := timestamp_before_tlbi mem in
+      let ts_to_check := if is_emptyb times then [max_t] else times in
+      foldlM (λ violated ttbr,
+        if (violated : bool) then mret true (* early return *)
+        else
+          snapshots ← mlift $
+            TLB.unique_snapshots_until ts initmem mem max_t ttbr;
+          mret $
+            existsb (λ '(tlb, time),
+              if decide (time ∉ ts_to_check) then false
+              else check_bbm_violation_in_snapshot mem initmem tlb time
+            ) snapshots
+      ) false (elements ttbrs_to_check)
+    else
+      mret false.
+End BBM.
 
 Module CProm.
   Record t :=
@@ -2056,6 +2332,9 @@ Section ComputeProm.
       run_to_termination_promise isem fuel base (CProm.init, PPState.Make ts mem IIS.init) in
     guard_or ("Out of fuel when searching for new promises")%string
       (∀ r ∈ res_proms, r.2 = true);;
+    guard_or ("BBM check fails")%string
+      (∀ st ∈ res_proms.*1.*2,
+        ∀ r ∈ (Exec.results $ check_bbm_violation initmem st), negb r.2);;
     let promises := res_proms.*1.*1 |> union_list |> CProm.proms in
     let tstates :=
       res_proms
